More SteelSel -> Steel renamings

ulib/experimental/Steel.Primitive.ForkJoin.Unix.fst
@@ -1,4 +1,4 @@
-module Steel.SelPrimitive.ForkJoin.Unix
+module Steel.Primitive.ForkJoin.Unix
 
 (* This module shows that it's possible to layer continuations on top
 of SteelT to get a direct style (or Unix style) fork/join. Very much a
@@ -6,10 +6,10 @@ prototype for now. *)
 
 open FStar.Ghost
 open Steel.Memory
-open Steel.SelEffect.Atomic
-open Steel.SelEffect
-open Steel.SelReference
-open Steel.SelPrimitive.ForkJoin
+open Steel.Effect.Atomic
+open Steel.Effect
+open Steel.Reference
+open Steel.Primitive.ForkJoin
 
 #set-options "--warn_error -330"  //turn off the experimental feature warning
 #set-options "--ide_id_info_off"
@@ -17,12 +17,12 @@ open Steel.SelPrimitive.ForkJoin
 // (* Some helpers *)
 let change_slprop_equiv (p q : vprop)
               (proof : squash (p `equiv` q))
-   : SteelSelT unit p (fun _ -> q)
+   : SteelT unit p (fun _ -> q)
    = rewrite_slprop p q (fun _ -> proof; reveal_equiv p q)
 
 let change_slprop_imp (p q : vprop)
               (proof : squash (p `can_be_split` q))
-   : SteelSelT unit p (fun _ -> q)
+   : SteelT unit p (fun _ -> q)
    = rewrite_slprop p q (fun _ -> proof; reveal_can_be_split ())
 
 (* Continuations into unit, but parametrized by the final heap
@@ -32,8 +32,8 @@ let change_slprop_imp (p q : vprop)
  * at least one of the branches. *)
 type steelK (t:Type u#aa) (framed:bool) (pre : vprop) (post:t->vprop) =
   #frame:vprop -> #postf:vprop ->
-  f:(x:t -> SteelSelT unit (frame `star` post x) (fun _ -> postf)) ->
-  SteelSelT unit (frame `star` pre) (fun _ -> postf)
+  f:(x:t -> SteelT unit (frame `star` post x) (fun _ -> postf)) ->
+  SteelT unit (frame `star` pre) (fun _ -> postf)
 
 (* The classic continuation monad *)
 let return_ a (x:a) (#[@@@ framing_implicit] p: a -> vprop) : steelK a true (return_pre (p x)) p =
@@ -81,7 +81,7 @@ let bind (a:Type) (b:Type)
     true
     (pre_f `star` frame_f)
     (fun y -> post_g y `star` frame_g)
-  = fun #frame (#post:vprop) (k:(y:b -> SteelSelT unit (frame `star` (post_g y `star` frame_g)) (fun _ -> post))) ->
+  = fun #frame (#post:vprop) (k:(y:b -> SteelT unit (frame `star` (post_g y `star` frame_g)) (fun _ -> post))) ->
     // Need SteelT unit (frame `star` (pre_f `star` frame_f)) (fun _ -> post)
     change_slprop_equiv (frame `star` (pre_f `star` frame_f)) ((frame `star` frame_f) `star` pre_f)  (rearrange3 frame frame_f pre_f;
         equiv_symmetric ((frame `star` frame_f) `star` pre_f) (frame `star` (pre_f `star` frame_f)) );
@@ -94,11 +94,11 @@ let bind (a:Type) (b:Type)
           (can_be_split_forall_frame (fun x -> post_f x `star` frame_f) (fun x -> pre_g x `star` frame_g) frame x);
         g x #(frame `star` frame_g) #post
           ((fun (y:b) -> k y)
-            <: (y:b -> SteelSelT unit ((frame `star` frame_g) `star` post_g y) (fun _ -> post)))
+            <: (y:b -> SteelT unit ((frame `star` frame_g) `star` post_g y) (fun _ -> post)))
 
         )
 
-      <: (x:a -> SteelSelT unit ((frame `star` frame_f) `star` post_f x) (fun _ -> post)))
+      <: (x:a -> SteelT unit ((frame `star` frame_f) `star` post_f x) (fun _ -> post)))
 
 let subcomp (a:Type)
   (#framed_f:eqtype_as_type bool) (#framed_g:eqtype_as_type bool)
@@ -108,11 +108,11 @@ let subcomp (a:Type)
   (#[@@@ framing_implicit] p2:squash (can_be_split_forall post_f post_g))
   (f:steelK a framed_f pre_f post_f)
 : Tot (steelK a framed_g pre_g post_g)
-= fun #frame #postf (k:(x:a -> SteelSelT unit (frame `star` post_g x) (fun _ -> postf))) ->
+= fun #frame #postf (k:(x:a -> SteelT unit (frame `star` post_g x) (fun _ -> postf))) ->
     change_slprop_imp pre_g pre_f (); f
       ((fun x -> change_slprop_imp (frame `star` post_f x) (frame `star` post_g x)
                             (can_be_split_forall_frame post_f post_g frame x);
-               k x) <: (x:a -> SteelSelT unit (frame `star` post_f x) (fun _ -> postf)))
+               k x) <: (x:a -> SteelT unit (frame `star` post_f x) (fun _ -> postf)))
 
 // let if_then_else (a:Type u#aa)
 //                  (#[@@@ framing_implicit] pre1:pre_t)
@@ -154,7 +154,7 @@ let bind_tot_steelK_ (a:Type) (b:Type)
     framed
     pre
     post
-  = fun #frame #postf (k:(x:b -> SteelSelT unit (frame `star` post x) (fun _ -> postf))) ->
+  = fun #frame #postf (k:(x:b -> SteelT unit (frame `star` post x) (fun _ -> postf))) ->
       let x = f () in
       g x k
 
@@ -168,7 +168,7 @@ let test_lift #p #q (f : unit -> SteelK unit p (fun _ -> q)) : SteelK unit p (fu
 
 (* Identity cont with frame, to eliminate a SteelK *)
 
-let idk (#frame:vprop) (#a:Type) (x:a) : SteelSelT a frame (fun x -> frame)
+let idk (#frame:vprop) (#a:Type) (x:a) : SteelT a frame (fun x -> frame)
   = noop(); return x
 
 let kfork (#p:vprop) (#q:vprop) (f : unit -> SteelK unit p (fun _ -> q))
@@ -176,14 +176,14 @@ let kfork (#p:vprop) (#q:vprop) (f : unit -> SteelK unit p (fun _ -> q))
 =
   SteelK?.reflect (
   fun (#frame:vprop) (#postf:vprop)
-    (k : (x:(thread q) -> SteelSelT unit (frame `star` emp) (fun _ -> postf))) ->
+    (k : (x:(thread q) -> SteelT unit (frame `star` emp) (fun _ -> postf))) ->
       noop ();
-      let t1 () : SteelSelT unit (emp `star` p) (fun _ -> q) =
+      let t1 () : SteelT unit (emp `star` p) (fun _ -> q) =
         let r : steelK unit false p (fun _ -> q) = reify (f ()) in
         r #emp #q (fun _ -> idk())
       in
-      let t2 (t:thread q) () : SteelSelT unit frame (fun _ -> postf) = k t in
-      let ff () : SteelSelT unit (p `star` frame) (fun _ -> postf) =
+      let t2 (t:thread q) () : SteelT unit frame (fun _ -> postf) = k t in
+      let ff () : SteelT unit (p `star` frame) (fun _ -> postf) =
         fork #p #q #frame #postf t1 t2
       in
       ff())
@@ -205,9 +205,9 @@ let example () : SteelK unit emp (fun _ -> q 1 `star` q 2) =
   h();
   kjoin p2
 
-let as_steelk_repr' (a:Type) (pre:pre_t) (post:post_t a) (f:unit -> SteelSelT a pre post)
+let as_steelk_repr' (a:Type) (pre:pre_t) (post:post_t a) (f:unit -> SteelT a pre post)
   : steelK a false pre post
-  = fun #frame #postf (k:(x:a -> SteelSelT unit (frame `star` post x) (fun _ -> postf))) ->
+  = fun #frame #postf (k:(x:a -> SteelT unit (frame `star` post x) (fun _ -> postf))) ->
       let x = f () in
       k x
 
@@ -218,7 +218,7 @@ let triv_post (#a:Type) (req:vprop) (ens:post_t a) : ens_t req a ens = fun _ _ _
 let as_steelk_repr (a:Type) (pre:pre_t) (post:post_t a)
   (f:repr a false pre post (triv_pre pre) (triv_post pre post))// unit -> SteelT a pre post)
   : steelK a false pre post
-  = as_steelk_repr' a pre post (fun _ -> SteelSelBase?.reflect f)
+  = as_steelk_repr' a pre post (fun _ -> SteelBase?.reflect f)
 
 // let as_steelk_repr' (a:Type) (pre:slprop) (post:post_t a) (f:unit -> SteelT a pre post)
 //   : steelK a pre post
@@ -232,14 +232,14 @@ let as_steelk_repr (a:Type) (pre:pre_t) (post:post_t a)
 
 open Steel.FractionalPermission
 
-sub_effect SteelSelBase ~> SteelKBase = as_steelk_repr
+sub_effect SteelBase ~> SteelKBase = as_steelk_repr
 
 let example2 (r:ref int) : SteelK (thread (pts_to r full_perm 1)) (pts_to r full_perm 0) (fun _ -> emp) =
   let p1 = kfork (fun _ -> write_pt #_ #0 r 1) in
   p1
 
 let alloc_pt (#a:Type) (x:a)
-  : SteelSelT (ref a) emp (fun r -> pts_to r full_perm x)
+  : SteelT (ref a) emp (fun r -> pts_to r full_perm x)
   = alloc_pt x
 
 let example3 (r:ref int) : SteelK (ref int) (pts_to r full_perm 0) (fun x -> pts_to r full_perm 1 `star` pts_to x full_perm 2) =
