ulib/experimental/Steel.Utils.fst
@@ -1,16 +1,16 @@
-module Steel.SelUtils
+module Steel.Utils
 open Steel.Memory
-open Steel.SelEffect.Atomic
-open Steel.SelEffect
+open Steel.Effect.Atomic
+open Steel.Effect
 open Steel.FractionalPermission
-open Steel.SelReference
+open Steel.Reference
 
 let pts_to_not_null (#a:Type)
                     (#opened:inames)
                     (#p:perm)
                     (#v:FStar.Ghost.erased a)
                     (r:ref a)
-  : SteelSelGhost unit opened
+  : SteelGhost unit opened
     (pts_to r p v)
     (fun _ -> pts_to r p v)
     (fun _ -> True)
@@ -20,7 +20,7 @@ let pts_to_not_null (#a:Type)
 
 let change_slprop_ens (p:vprop) (q:vprop) (r:prop) (f:(m:mem -> Lemma (requires interp (hp_of p) m)
                                                                        (ensures interp (hp_of q) m /\ r)))
-  : SteelSel unit p (fun _ -> q) (requires fun _ -> True) (ensures fun _ _ _ -> r)
+  : Steel unit p (fun _ -> q) (requires fun _ -> True) (ensures fun _ _ _ -> r)
   = rewrite_slprop p (q `star` pure r)
                                  (fun m -> f m;
                                         Steel.Memory.emp_unit (hp_of q);
@@ -28,22 +28,22 @@ let change_slprop_ens (p:vprop) (q:vprop) (r:prop) (f:(m:mem -> Lemma (requires 
     elim_pure r
 
 let pure_as_ens (#p:prop) ()
-  : SteelSel unit (pure p) (fun _ -> pure p) (fun _ -> True) (fun _ _ _ -> p)
+  : Steel unit (pure p) (fun _ -> pure p) (fun _ -> True) (fun _ _ _ -> p)
   = change_slprop_ens (pure p) (pure p) p (Steel.Memory.pure_interp p)
 
 let rewrite #a (#p:a -> vprop) (x y:a)
-  : SteelSel unit (p x) (fun _ -> p y)
+  : Steel unit (p x) (fun _ -> p y)
     (requires fun _ -> x == y)
     (ensures fun _ _ _ -> True)
   = rewrite_slprop (p x) (p y) (fun _ -> ())
 
 let extract_pure (p:prop)
-  : SteelSel unit (pure p) (fun _ -> pure p) (fun _ -> True) (fun _ _ _ -> p)
+  : Steel unit (pure p) (fun _ -> pure p) (fun _ -> True) (fun _ _ _ -> p)
   = elim_pure p;
     intro_pure p
 
 let dup_pure (p:prop)
-  : SteelSelT unit (pure p) (fun _ -> pure p `star` pure p)
+  : SteelT unit (pure p) (fun _ -> pure p `star` pure p)
   = extract_pure p;
     intro_pure p
 
